Sodium/Crypto/Stream.lean
@@ -1,4 +1,3 @@
-import Sodium.Data.AsyncList
 import Sodium.Data.Chunk
 import Sodium.Crypto.Monad
 
@@ -12,80 +11,57 @@ variable {α ε σ : Type} {τ : Sodium σ}
 
 structure SecretEncoder (τ : Sodium σ) where
   private mk ::
-  closed : IO.Ref Bool
   header : Header XChaCha20Poly1305
-  stream : SecureStream τ
+  stream : SecretStream τ
 
 namespace SecretEncoder
 
 def new (key : Option (SymmKey τ XChaCha20) := none) : CryptoM τ (SecretEncoder τ) := do
   let key ← key.getDM (mkStaleKey (·.cast))
   let (stream, header) ← streamInitPush (key.cast (by simp [USize.ofNatLT_eq_ofNat]; congr))
-  let closed ← IO.mkRef false
-  return {stream, header := header.cast, closed}
+  return {stream, header := header.cast}
 
-def isClosed (encoder : SecretEncoder τ) : CryptoM τ Bool :=
-  encoder.closed.get
-
-def close (encoder : SecretEncoder τ) : CryptoM τ Unit :=
-  encoder.closed.set true
-
-def push [ToChunks α] (encoder : SecretEncoder τ) (x : α) (prio : Task.Priority := .dedicated) (final := false) : CryptoM τ (IO.AsyncList IO.Error (CipherChunk XChaCha20Poly1305)) := do
+def push [ToChunks α] (encoder : SecretEncoder τ) (x : α) (final := false) : CryptoM τ (List (CipherChunk XChaCha20Poly1305)) := do
   have : XChaCha20Poly1305.shapeOf `mac = ABYTES := by native_decide
-  if ← encoder.closed.get then return ∅
   let chunks := toChunks x |>.map (String.toUTF8 ∘ Json.compress)
   let some last := chunks.getLast?
     | return ∅
-  let messages ← chunks.dropLast.foldIO (prio := prio) fun chunk => do
+  let messages ← chunks.dropLast.mapM fun chunk => do
     let cipher ← streamPush encoder.stream chunk.toVector .empty .message
     return ⟨cipher.size, cipher, by simp [this]⟩
-  let terminal ← Server.ServerTask.IO.asTask <| do
-    let cipher ← streamPush encoder.stream last.toVector .empty (if final then .final else .push)
-    return ⟨cipher.size, cipher, by simp [this]⟩
-  if final then encoder.closed.set true
-  return messages.append <| .delayed <| terminal.mapCheap (·.map pure)
+  let terminal ← streamPush encoder.stream last.toVector .empty (if final then .final else .push)
+  return messages ++ [⟨terminal.size, terminal, by simp [this]⟩]
 
-def rekey (encoder : SecretEncoder τ) : CryptoM τ (IO.AsyncList IO.Error (CipherChunk XChaCha20Poly1305)) := do
+def rekey (encoder : SecretEncoder τ) : CryptoM τ (List (CipherChunk XChaCha20Poly1305)) := do
   have : XChaCha20Poly1305.shapeOf `mac = ABYTES := by native_decide
-  if ← encoder.closed.get then return ∅
   let cipher ← streamPush encoder.stream (json% null).compress.toUTF8.toVector .empty .rekey
   streamRekey encoder.stream
-  return .ofList [⟨cipher.size, cipher, by simp [this]⟩]
+  return [⟨cipher.size, cipher, by simp [this]⟩]
 
 end SecretEncoder
 
 structure SecretDecoder (τ : Sodium σ) where
   private mk ::
-  closed : IO.Ref Bool
-  buffer : IO.Ref (List Json)
-  stream : SecureStream τ
+  buffer : IO.Ref (Array Json)
+  stream : SecretStream τ
 
 namespace SecretDecoder
 
 def new (header : Header XChaCha20Poly1305) (key : Option (SymmKey τ XChaCha20) := none) : CryptoM τ (SecretDecoder τ) := do
   let key ← key.getDM (mkStaleKey (·.cast))
   let stream ← streamInitPull header.cast (key.cast (by simp [USize.ofNatLT_eq_ofNat]; congr))
-  let buffer ← IO.mkRef []
-  let closed ← IO.mkRef false
-  return {stream, buffer, closed}
+  let buffer ← IO.mkRef #[]
+  return {stream, buffer}
 
-def isClosed (decoder : SecretDecoder τ) : CryptoM τ Bool :=
-  decoder.closed.get
-
-def close (decoder : SecretDecoder τ) : CryptoM τ Unit :=
-  decoder.closed.set true
-
-def pull [FromChunks α] (decoder : SecretDecoder τ) (src : List (CipherChunk XChaCha20Poly1305)) : CryptoM τ (List α × Option DecryptError) := do
-  if ← decoder.closed.get then return ([], some .refused)
-  let mut results : List α := []
+def pull [FromChunks α] (decoder : SecretDecoder τ) (src : List (CipherChunk XChaCha20Poly1305)) : CryptoM τ (Array α × Option DecryptError) := do
+  let mut results : Array α := #[]
   let mut error : Option DecryptError := none
 
   for chunk in src do
-    if ← decoder.closed.get then break
     if error.isSome then break
 
     have : chunk.size = ABYTES + (chunk.size - ABYTES) := by
-      have mac_le : XChaCha20Poly1305.shapeOf `mac ≤ chunk.size := chunk.shapeOf_mac_le_size
+      have mac_le : XChaCha20Poly1305.shapeOf `mac ≤ chunk.size := chunk.mac_le_size
       have : XChaCha20Poly1305.shapeOf `mac = ABYTES := by native_decide
       rw [this] at mac_le
       rw [Nat.add_comm, Nat.sub_add_cancel mac_le]
@@ -103,20 +79,15 @@ def pull [FromChunks α] (decoder : SecretDecoder τ) (src : List (CipherChunk X
         break
 
     match tag with
-    | .rekey =>
-      streamRekey decoder.stream
-    | .message => decoder.buffer.modify fun acc => acc ++ [json]
-    | .push =>
-      let acc := (← decoder.buffer.swap []) ++ [json]
-      match fromChunks? acc with
-      | .ok item => results := results ++ [item]
-      | .error msg => error := some (.invalidJson (Json.arr acc.toArray))
-    | .final =>
-      decoder.closed.set true
-      let acc := (← decoder.buffer.swap []) ++ [json]
-      match fromChunks? acc with
-      | .ok item => results := results ++ [item]
-      | .error msg => error := some (.invalidJson (Json.arr acc.toArray))
+    | .rekey => streamRekey decoder.stream
+    | .message => decoder.buffer.modify (·.push json)
+    | .push | .final =>
+      let acc := (← decoder.buffer.swap #[]).push json
+      match fromChunks? acc.toList with
+      | some item => results := results.push item
+      | _ => error := some (.invalidJson (Json.arr acc))
+
+    if tag = .final then break
 
   return (results, error)
 
