Sodium.lean
@@ -1,9 +1,12 @@
 import «Sodium».Crypto.Monad
 import «Sodium».Data.Digest
+import «Sodium».Lean.Syntax
 
 open Lean Sodium Crypto
 
-#eval show MetaM Json from CryptoM.toMetaM fun _ => do
-  let sig ← sign (json% {some: "string"})
-  println! digest sig
-  return encode sig
+#eval show MetaM Format from CryptoM.toMetaM fun _ => do
+  let stx ← TSyntax.encodable.syntax `tactic
+  let x ← encrypt stx
+  let .accepted y ← decrypt? (α := TSyntax ``Lean.Parser.Tactic.tacticSeq) x
+    | return default
+  return y.raw.prettyPrint
