Sodium/Data/Chunk.lean
@@ -1,5 +1,6 @@
 import Lean.Data.Json
 import Sodium.Data.ByteArray
+import Sodium.Data.Encodable.Basic
 
 universe u
 
@@ -12,25 +13,25 @@ class ToChunks (α : Type u) where
 
 export ToChunks (toChunks)
 
-instance [ToJson α] : ToChunks (List α) where
-  toChunks xs := xs.map toJson
+instance [Encodable α] : ToChunks (List α) where
+  toChunks xs := xs.map encode
 
-instance [ToJson α] : ToChunks (Array α) := ⟨toChunks ∘ Array.toList⟩
+instance [Encodable α] : ToChunks (Array α) := ⟨toChunks ∘ Array.toList⟩
 
 class FromChunks (α : Type u) where
-  fromChunks? : List Json → Except String α
+  fromChunks? : List Json → Option α
 
 export FromChunks (fromChunks?)
 
 class LawfulChunks (α : Type u) [ToChunks α] [FromChunks α] where
-  chunksk : ∀ a, fromChunks? (α := α) (toChunks a) = .ok a
+  chunksk : ∀ a, fromChunks? (α := α) (toChunks a) = some a
 
-instance [FromJson α] : FromChunks (List α) where
+instance [Encodable α] : FromChunks (List α) where
   fromChunks?
-    | [] => .ok []
-    | chunks => chunks.mapM fromJson?
+    | [] => some []
+    | chunks => chunks.mapM decode?
 
-instance [FromJson α] : FromChunks (Array α) := ⟨fun xs => fromChunks? xs |>.map List.toArray⟩
+instance [Encodable α] : FromChunks (Array α) := ⟨fun xs => fromChunks? xs |>.map List.toArray⟩
 
 namespace ByteArray
 
@@ -42,21 +43,21 @@ instance : ToChunks ByteArray where
     while !cursor.atEnd do
       let len := min 12288 cursor.remainingBytes
       let buf := cursor.array.extract cursor.pos (cursor.pos + len)
-      chunks := chunks.push (toJson buf)
+      chunks := chunks.push (encode buf)
       cursor := cursor.forward len
     return chunks.toList
 
 instance : FromChunks ByteArray where
   fromChunks?
-    | [] => .ok .empty
+    | [] => some .empty
     | chunks => do
       let capacity := chunks.length * 12288
       let mut buf := ByteArray.emptyWithCapacity capacity
       let mut idx := 0
       for chunk in chunks do
-        match fromJson? (α := ByteArray) chunk with
-        | .error e => throw e
-        | .ok bytes =>
+        match decode? chunk with
+        | none => none
+        | some bytes =>
           buf := bytes.copySlice
             (srcOff := 0)
             (dest := buf)
