Sodium/Data/PFunctor.lean
@@ -1,0 +1,96 @@
+import Sodium.Data.Encodable.WType
+
+universe u v w uα uβ uγ uδ
+
+structure PFunctor where
+  A : Type u
+  B : A → Type v
+
+namespace PFunctor
+
+variable {α : Type u} {β : Type v} {γ : Type w}
+
+@[coe] def new (P : PFunctor.{uα,uβ}) (α : Type u) : Type (max u uα uβ) :=
+  Σ x : P.A, P.B x → α
+
+protected abbrev Id (P : PFunctor.{uα, uβ}) : Type (max uα uβ) :=
+  Σ x : P.A, P.B x
+
+instance : CoeFun PFunctor.{uα,uβ} (fun _ => Type u → Type (max u uα uβ)) := ⟨new⟩
+
+instance : Inhabited PFunctor.{uα,uβ} := ⟨⟨default, default⟩⟩
+
+variable (P : PFunctor.{uα,uβ})
+
+instance [Inhabited P.A] [Inhabited α] : Inhabited (P α) := ⟨⟨default, default⟩⟩
+instance [Inhabited P.A] [Inhabited (P.B default)] : Inhabited P.Id := ⟨⟨default, default⟩⟩
+
+instance [Encodable P.A] [∀ a, Encodable (P.B a)] : Encodable P.Id := by unfold PFunctor.Id; infer_instance
+
+def map (f : α → β) : P α → P β := fun ⟨a, g⟩ => ⟨a, f ∘ g⟩
+
+instance : Functor P.new where map := P.map
+
+@[simp] theorem map_eq_map {α β : Type u} (f : α → β) (x : P α) : f <$> x = P.map f x := rfl
+@[simp] theorem map_eq (f : α → β) (a : P.A) (g : P.B a → α) : P.map f ⟨a, g⟩ = ⟨a, f ∘ g⟩ := rfl
+@[simp] theorem id_map : ∀ x : P α, P.map id x = x := fun ⟨_, _⟩ => rfl
+@[simp] theorem map_map (f : α → β) (g : β → γ) : ∀ x : P α, P.map g (P.map f x) = P.map (g ∘ f) x := fun ⟨_, _⟩ => rfl
+
+instance : LawfulFunctor P.new where
+  map_const := rfl
+  id_map x := P.id_map x
+  comp_map f g x := P.map_map f g x |>.symm
+
+abbrev W : Type (max uα uβ) := @WType P.A P.B
+
+variable {P}
+
+def W.head : P.W → P.A
+  | ⟨a, _⟩ => a
+
+def W.children : ∀ x : P.W, P.B (W.head x) → P.W
+  | ⟨_, f⟩ => f
+
+def W.next : P.W → P P.W
+  | ⟨a, f⟩ => ⟨a, f⟩
+
+def W.mk : P P.W → P.W
+  | ⟨a, f⟩ => ⟨a, f⟩
+
+@[simp] theorem W.next_mk (p : P P.W) : W.next (W.mk p) = p := by cases p; rfl
+@[simp] theorem W.mk_next (p : P.W) : W.mk (W.next p) = p := by cases p; rfl
+
+def new.iget [DecidableEq P.A] [Inhabited α] (x : P α) (i : P.Id) : α :=
+  if h : i.1 = x.1 then x.2 (cast (congrArg _ h) i.2) else default
+
+@[simp] theorem fst_map (x : P α) (f : α → β) : (P.map f x).1 = x.1 := by cases x; rfl
+
+@[simp] theorem iget_map [DecidableEq P.A] [Inhabited α] [Inhabited β] (x : P α)
+    (f : α → β) (i : P.Id) (h : i.1 = x.1) : (P.map f x).iget i = f (x.iget i) := by
+  simp only [new.iget, fst_map, *]
+  cases x
+  rfl
+
+def comp (P₂ : PFunctor.{uγ,uδ}) (P₁ : PFunctor.{uα,uβ}) : PFunctor.{max uα uγ uδ, max uβ uδ} where
+  A := Σ a₂ : P₂.A, P₂.B a₂ → P₁.A
+  B | ⟨a, k⟩ => Σ u : P₂.B a, P₁.B (k u)
+
+notation a " ⊚ " b => comp a b
+
+def comp.mk (P₂ : PFunctor.{uγ,uδ}) (P₁ : PFunctor.{uα,uβ}) {α : Type u} (x : P₂ (P₁ α)) : comp P₂ P₁ α :=
+  ⟨⟨x.1, Sigma.fst ∘ x.2⟩, fun ⟨a, k⟩ => (x.2 a).2 k⟩
+
+def comp.get (P₂ : PFunctor.{uγ,uδ}) (P₁ : PFunctor.{uα,uβ}) {α : Type u} (x : comp P₂ P₁ α) : P₂ (P₁ α) :=
+  ⟨x.1.1, fun a₂ => ⟨x.1.2 a₂, fun a₁ => x.2 ⟨a₂, a₁⟩⟩⟩
+
+protected def W.cases {X : P.W → Sort w} (f : ∀ x : P P.W, X (W.mk x)) (p : P.W) : X p :=
+  suffices X (W.mk (W.next p)) by
+    rw [← W.mk_next p]
+    exact this
+  f _
+
+@[simp] theorem W.cases_mk {X : P.W → Sort w} (p : P P.W) (f : ∀ x : P P.W, X (W.mk x)) : W.cases f (W.mk p) = f p := by
+  simp only [W.mk, W.cases, W.next]
+  cases p; simp only [eq_mpr_eq_cast, cast_eq]
+
+end PFunctor
