Sodium/Server/Monad.lean
@@ -1,0 +1,132 @@
+import Sodium.Server.Types
+
+open Lean Sodium Crypto
+
+namespace Sodium.Server
+
+export Lean.Server (ServerTask)
+
+variable {α β σ : Type} {τ : Sodium σ} {m : {σ : Type} → Sodium σ → Type → Type}
+
+def Server (α : Type) := Message (BaseIO (ServerTask α))
+
+namespace Server
+
+def ephemeral (x : BaseIO (ServerTask α)) : Server α :=
+  ⟨.ephemeral, fun _ => x⟩
+
+def addressed (x : Message.B .addressed → BaseIO (ServerTask α)) : Server α :=
+  ⟨.addressed, x⟩
+
+def anonymous (x : Message.B .anonymous → BaseIO (ServerTask α)) : Server α :=
+  ⟨.anonymous, x⟩
+
+end Server
+
+def ServerT (τ : Sodium σ) (m : {σ : Type} → Sodium σ → Type → Type) (α : Type) :=
+  Message (m τ α)
+
+namespace ServerT
+
+instance : Inhabited (ServerT τ m α) := by unfold ServerT; infer_instance
+
+def ephemeral (x : m τ α) : ServerT τ m α :=
+  ⟨.ephemeral, fun _ => x⟩
+
+def anonymous (x : Message.B .anonymous → m τ α) : ServerT τ m α :=
+  ⟨.anonymous, x⟩
+
+def addressed (x : Message.B .addressed → m τ α) : ServerT τ m α :=
+  ⟨.addressed, x⟩
+
+protected def pure [Pure (m τ)] (a : α) : ServerT τ m α :=
+  ephemeral (Pure.pure a)
+
+protected def map [Functor (m τ)] (f : α → β) : ServerT τ m α → ServerT τ m β :=
+  Message.map (Functor.map f)
+
+protected def bind [h : Monad (m τ)] [MonadError (m τ)] (st : ServerT τ m α) (f : α → ServerT τ m β) : ServerT τ m β :=
+  match st with | ⟨ka, k⟩ => by refine ⟨ka, ?_⟩; exact fun x => do
+    bind (k x) fun a => match f a with
+      | ⟨.ephemeral, k⟩ => k ()
+      | ⟨msg, k⟩ =>
+        if h : msg = ka then k (h ▸ x)
+        else throwError toMessageData (@toJson MessageKind _ msg)
+
+instance [Functor (m τ)] : Functor (ServerT τ m) where map := ServerT.map
+
+instance [Monad (m τ)] [MonadError (m τ)] : Monad (ServerT τ m) where
+  pure := ServerT.pure
+  bind := ServerT.bind
+
+variable [Monad (m τ)] [MonadError (m τ)]
+
+def run (x : Message.Id) : ServerT τ m α → m τ α
+  | ⟨.ephemeral, k⟩ => k ()
+  | ⟨a, k⟩ =>
+    if h : a = x.1 then k (h ▸ x.2)
+    else throwError toMessageData (@toJson MessageKind _ a)
+
+end ServerT
+
+structure ServerContext (τ : Sodium σ) where
+  session : Option (Session τ Curve25519Blake2b) := none
+
+abbrev ServerM (τ : Sodium σ) := ReaderT (ServerContext τ) (ServerT τ CryptoM)
+
+namespace ServerM
+
+def toCryptoM (msg : Message.Id) (x : ServerM τ α) (session : Option (Session τ Curve25519Blake2b) := none) : CryptoM τ α :=
+  ServerT.run msg (x {session})
+
+def recv? (α : Type) [Encodable α] : ServerM τ (Decrypt (Verified α))
+  | { session := none } => ServerT.anonymous fun x => do decryptAnon? x
+  | { session := some session } => ServerT.addressed fun x =>
+    session.withReceiver do
+      match ← decrypt? x with
+      | .accepted a => return .accepted (← sign a)
+      | .almost json => return .almost json
+      | .unknown str => return .unknown str
+      | .mangled bytes => return .mangled bytes
+      | .refused => return .refused
+
+def recv! (α : Type) [Encodable α] : ServerM τ (Verified α) := do
+  let .accepted x ← recv? α | default
+  return x
+
+def recvFrom? (α : Type) [Encodable α] (pkey : MachineId) : ServerM τ (Decrypt (Verified α))
+  | { session := none } => ServerT.anonymous fun x => do
+    let some key ← newSharedKey? pkey | throwSpecViolation Curve25519 `publickey
+    withSharedKey key do decryptAnon? x
+  | { session := some session } => ServerT.addressed fun x => do
+    session.withReceiver do
+      let some key ← newSharedKey? pkey | throwSpecViolation Curve25519 `publickey
+      match ← decryptFrom? key x with
+      | .accepted a => return .accepted (← sign a)
+      | .almost json => return .almost json
+      | .unknown str => return .unknown str
+      | .mangled bytes => return .mangled bytes
+      | .refused => return .refused
+
+def recvFrom! (α : Type) [Encodable α] (pkey : MachineId) : ServerM τ (Verified α) := do
+  let .accepted x ← recvFrom? α pkey | default
+  return x
+
+def send {α : Type} [Encodable α] (a : α) : Server β → ServerM τ (ServerTask β)
+  | ⟨.ephemeral, k⟩, _ => ServerT.ephemeral do k ()
+  | ⟨.addressed, k⟩, {session} => ServerT.ephemeral do (session.map (·.withTransmitter)).getD id do k (← encrypt a)
+  | _, _ => default
+
+def sendTo {α : Type} [Encodable α] (pkey : MachineId) (a : α) : Server β → ServerM τ (ServerTask β)
+  | ⟨.ephemeral, k⟩, _ => ServerT.ephemeral do k ()
+  | ⟨.anonymous, k⟩, {session} => ServerT.ephemeral do (session.map (·.withTransmitter)).getD id do
+    let some msg ← encryptAnon? pkey a | throwSpecViolation Curve25519 `publickey
+    k msg
+  | ⟨.addressed, k⟩, {session} => ServerT.ephemeral do (session.map (·.withTransmitter)).getD id do
+    let some key ← newSharedKey? pkey | throwSpecViolation Curve25519 `publickey
+    k (← encryptTo key a)
+  | _, _ => default
+
+end ServerM
+
+end Sodium.Server
