Sodium/Server/Types.lean
@@ -1,0 +1,139 @@
+import Sodium.Crypto.Monad
+import Sodium.Data.PFunctor
+import Sodium.Lean.Syntax
+
+open Lean Sodium Crypto
+
+variable {σ : Type} {τ : Sodium σ}
+
+namespace Sodium.Server
+
+abbrev MachineId := Verified (PublicKey Curve25519)
+
+abbrev AgentId := Verified (PublicKey Ed25519)
+
+structure PeerId extends AgentId where
+  self_signed : pkey = val
+
+namespace PeerId
+
+def new (keys : Option (KeyPair τ Ed25519) := none) : CryptoM τ PeerId := do
+  let keys ← keys.getDM mkStaleSignature
+  let sig ← sign keys.pkey keys
+  if h : sig.pkey = sig.val then return ⟨sig, h⟩
+  throwSpecViolation Ed25519 `publickey
+
+instance encodable : Encodable PeerId :=
+  Encodable.ofEquiv {x : AgentId // x.pkey = x.val} {
+    push := fun ⟨x, h⟩ => ⟨x, h⟩
+    pull := fun ⟨x, h⟩ => ⟨x, h⟩
+  }
+
+class Signed {α : Type} [Encodable α] (p : PeerId) (x : Verified α) : Prop where
+  signed : p.pkey = x.pkey
+
+end PeerId
+
+structure FriendId (τ : Sodium σ) extends AgentId where
+  keys : KeyPair τ Ed25519
+  signed_with_held_secret : keys.pkey = pkey
+  exists_peer : ∃ peer : PeerId, peer.pkey = val
+
+namespace FriendId
+
+def new (peer : PeerId) (keys : Option (KeyPair τ Ed25519) := none) : CryptoM τ (FriendId τ) := do
+  let keys ← keys.getDM mkStaleSignature
+  let sig ← sign peer.pkey keys
+  if h : keys.pkey = sig.pkey ∧ peer.pkey = sig.val then return ⟨sig, keys, h.1, by constructor; exact h.2⟩
+  throwSpecViolation Ed25519 `publickey
+
+class Signed {α : Type} [Encodable α] (f : FriendId τ) (x : Verified α) : Prop where
+  signed : f.pkey = x.pkey
+
+end FriendId
+
+structure MetaId (τ : Sodium σ) extends PeerId, FriendId τ
+
+namespace MetaId
+
+def new (keys : Option (KeyPair τ Ed25519) := none) : CryptoM τ (MetaId τ) := do
+  let keys ← keys.getDM mkStaleSignature
+  let peer ← PeerId.new keys
+  if h : keys.pkey = peer.pkey then return ⟨peer, keys, h, by constructor; exact peer.self_signed⟩
+  throwSpecViolation Ed25519 `publickey
+
+class Signed {α : Type} [Encodable α] (m : MetaId τ) (x : Verified α) : Prop where
+  signed : m.pkey = x.pkey
+
+end MetaId
+
+inductive MessageKind
+  | terminal
+  | anonymous
+  | addressed
+  | «partial»
+  | ephemeral
+  deriving Inhabited, BEq, DecidableEq, Repr, TypeName, ToJson, FromJson
+
+namespace MessageKind
+
+def ofFin : Fin 5 → MessageKind
+  | 0 => .terminal
+  | 1 => .anonymous
+  | 2 => .addressed
+  | 3 => .partial
+  | 4 => .ephemeral
+
+@[coe] def toFin : MessageKind → Fin 5
+  | .terminal => 0
+  | .anonymous => 1
+  | .addressed => 2
+  | .partial => 3
+  | .ephemeral => 4
+
+@[simp] theorem ofFin_toFin_eq : ∀ k, ofFin (toFin k) = k := by intro k; cases k <;> rfl
+
+instance : Coe MessageKind (Fin 5) := ⟨toFin⟩
+
+instance encodable : Encodable MessageKind :=
+  Encodable.ofEquiv _ {
+    push := toFin
+    pull := ofFin
+    push_pull_eq k := ofFin_toFin_eq k
+  }
+
+end MessageKind
+
+def Message : PFunctor where
+  A := MessageKind
+  B | .terminal => Empty
+    | .anonymous => SealedCipherText Curve25519XSalsa20Poly1305
+    | .addressed => CipherText XSalsa20Poly1305
+    | .partial => List (CipherChunk XChaCha20Poly1305)
+    | .ephemeral => Unit
+
+namespace Message
+
+instance : Coe Message.A MessageKind := ⟨id⟩
+instance : Inhabited Message.A := by unfold Message; infer_instance
+instance : DecidableEq Message.A := by unfold Message; infer_instance
+
+instance {α} : Inhabited (Message α) := ⟨⟨default, Empty.elim⟩⟩
+instance : Inhabited Message.Id := ⟨⟨.ephemeral, ()⟩⟩
+
+instance encodable : Encodable Message.A := by unfold Message; infer_instance
+
+instance : IsEmpty (Message.B default) := by unfold Message; simp [instInhabitedA]; infer_instance
+
+instance : ∀ a, HEq (Message.B a) (Message.B a) := fun _ => by
+  simp only [heq_eq_eq]
+
+instance encodable_pi : ∀ a, Encodable (Message.B a) := fun a => by
+  have : Encodable Empty := Empty.encodable
+  cases a <;> unfold Message <;> simp only <;> infer_instance
+
+instance encodable_id : Encodable Message.Id := by infer_instance
+
+end Message
+
+end Sodium.Server
